examples/delayed_echo/Stack1.v
@@ -31,7 +31,7 @@ Section PROOF.
     end
   .
 
-  Let pop_spec: fspec := (mk_simple "LinkedList"
+  Let pop_spec: fspec := (mk_simple "Stack"
                                     (fun '(llref, xs) varg o =>
                                        Exists ll, ⌜varg = [Vptr llref 0%Z]↑⌝ ** Own (GRA.embed ((llref,0%Z) |-> [ll])) ** (is_list ll xs) ** ⌜o = ord_pure 2⌝)
                                     (fun '(llref, xs) vret =>
@@ -41,7 +41,7 @@ Section PROOF.
                                        end)
                          ).
 
-  Let pop2_spec: fspec := (mk_simple "LinkedList"
+  Let pop2_spec: fspec := (mk_simple "Stack"
                                      (fun '(xs, nref) varg o => Exists ll, ⌜varg = [ll; Vptr nref 0%Z]↑⌝ ** (is_list ll xs) **
                                                                            (Exists v, Own (GRA.embed ((nref, 0%Z) |-> [v]))) ** ⌜o = ord_pure 2⌝)
                                      (fun '(xs, nref) vret =>
@@ -62,33 +62,33 @@ Section PROOF.
 (*   return NULL; *)
 (* } *)
 
-  Let push_spec: fspec := (mk_simple "LinkedList"
+  Let push_spec: fspec := (mk_simple "Stack"
                                      (fun '(x, xs) varg o => Exists ll, ⌜varg = [ll; x]↑⌝ ** is_list ll xs ** ⌜o = ord_pure 2⌝)
                                      (fun '(x, xs) vret => Exists ll', is_list ll' (x :: xs) ** ⌜vret = ll'↑⌝)).
 
-  Definition LinkedListStb: list (gname * fspec).
+  Definition StackStb: list (gname * fspec).
     eapply (Seal.sealing "stb").
     apply [("pop", pop_spec) ; ("pop2", pop2_spec) ; ("push", push_spec)].
   Defined.
 
-  Definition LinkedListSbtb: list (gname * fspecbody) :=
+  Definition StackSbtb: list (gname * fspecbody) :=
     [("pop", mk_specbody pop_spec (fun _ => APC;; trigger (Choose _)));
     ("pop2", mk_specbody pop2_spec (fun _ => APC;; trigger (Choose _)));
     ("push",   mk_specbody push_spec (fun _ => APC;; trigger (Choose _)))
     ]
   .
 
-  Definition LinkedListSem: ModSem.t := {|
-    ModSem.fnsems := List.map (fun '(fn, fsb) => (fn, fun_to_tgt (MemStb ++ LinkedListStb) fn fsb)) LinkedListSbtb;
-    ModSem.initial_mrs := [("LinkedList", (ε, tt↑))];
+  Definition StackSem: ModSem.t := {|
+    ModSem.fnsems := List.map (fun '(fn, fsb) => (fn, fun_to_tgt (MemStb ++ StackStb) fn fsb)) StackSbtb;
+    ModSem.initial_mrs := [("Stack", (ε, tt↑))];
   |}
   .
 
-  Definition LinkedList: Mod.t := {|
-    Mod.get_modsem := fun _ => LinkedListSem;
+  Definition Stack: Mod.t := {|
+    Mod.get_modsem := fun _ => StackSem;
     Mod.sk := Sk.unit;
   |}
   .
 
 End PROOF.
-Global Hint Unfold LinkedListStb: stb.
+Global Hint Unfold StackStb: stb.
