examples/bw/BWMain1.v
@@ -6,7 +6,7 @@ Require Import ModSem.
 Require Import Skeleton.
 Require Import PCM.
 Require Import HoareDef.
-Require Import LinkedList1 Client1 BW1.
+Require Import Stack1 Client1 BW1.
 Require Import TODO TODOYJ.
 
 Set Implicit Arguments.
